theories/zoo_saturn/ws_bqueue_1__opaque.v
@@ -3,6 +3,8 @@ From zoo_saturn Require Import
 
 #[global] Opaque ws_bqueue_1_create.
 #[global] Opaque ws_bqueue_1_capacity.
+#[global] Opaque ws_bqueue_1_size.
+#[global] Opaque ws_bqueue_1_is_empty.
 #[global] Opaque ws_bqueue_1_push.
 #[global] Opaque ws_bqueue_1_pop.
 #[global] Opaque ws_bqueue_1_steal.
